git/leanprover/lean4/stage0/stdlib/Init/Prelude.c
@@ -7309,7 +7309,7 @@ static lean_object* _init_l_Lean_strLitKind___closed__1() {
 _start:
 {
 lean_object* x_1; 
-x_1 = lean_mk_string("strLit");
+x_1 = lean_mk_string("str");
 return x_1;
 }
 }
@@ -7335,7 +7335,7 @@ static lean_object* _init_l_Lean_charLitKind___closed__1() {
 _start:
 {
 lean_object* x_1; 
-x_1 = lean_mk_string("charLit");
+x_1 = lean_mk_string("char");
 return x_1;
 }
 }
@@ -7361,7 +7361,7 @@ static lean_object* _init_l_Lean_numLitKind___closed__1() {
 _start:
 {
 lean_object* x_1; 
-x_1 = lean_mk_string("numLit");
+x_1 = lean_mk_string("num");
 return x_1;
 }
 }
@@ -7387,7 +7387,7 @@ static lean_object* _init_l_Lean_scientificLitKind___closed__1() {
 _start:
 {
 lean_object* x_1; 
-x_1 = lean_mk_string("scientificLit");
+x_1 = lean_mk_string("scientific");
 return x_1;
 }
 }
@@ -7413,7 +7413,7 @@ static lean_object* _init_l_Lean_nameLitKind___closed__1() {
 _start:
 {
 lean_object* x_1; 
-x_1 = lean_mk_string("nameLit");
+x_1 = lean_mk_string("name");
 return x_1;
 }
 }
