git/leanprover/lean4/stage0/stdlib/Lean/Elab/BuiltinTerm.c
@@ -2637,7 +2637,7 @@ x_14 = l_Lean_Name_isAnonymous(x_13);
 if (x_14 == 0)
 {
 uint8_t x_15; 
-x_15 = lean_ctor_get_uint8(x_3, sizeof(void*)*7 + 6);
+x_15 = lean_ctor_get_uint8(x_3, sizeof(void*)*8 + 6);
 if (x_15 == 0)
 {
 lean_object* x_16; lean_object* x_17; lean_object* x_18; lean_object* x_19; lean_object* x_20; lean_object* x_21; lean_object* x_22; 
@@ -3290,7 +3290,7 @@ return x_167;
 else
 {
 uint8_t x_168; 
-x_168 = lean_ctor_get_uint8(x_3, sizeof(void*)*7 + 6);
+x_168 = lean_ctor_get_uint8(x_3, sizeof(void*)*8 + 6);
 if (x_168 == 0)
 {
 uint8_t x_169; lean_object* x_170; lean_object* x_171; lean_object* x_172; lean_object* x_173; lean_object* x_174; uint8_t x_175; 
@@ -5901,7 +5901,7 @@ static lean_object* _init_l___regBuiltin_Lean_Elab_Term_elabStrLit___closed__1()
 _start:
 {
 lean_object* x_1; 
-x_1 = lean_mk_string("strLit");
+x_1 = lean_mk_string("str");
 return x_1;
 }
 }
@@ -5958,7 +5958,7 @@ _start:
 {
 lean_object* x_1; lean_object* x_2; lean_object* x_3; 
 x_1 = lean_unsigned_to_nat(165u);
-x_2 = lean_unsigned_to_nat(26u);
+x_2 = lean_unsigned_to_nat(23u);
 x_3 = lean_alloc_ctor(0, 2, 0);
 lean_ctor_set(x_3, 0, x_1);
 lean_ctor_set(x_3, 1, x_2);
@@ -5982,7 +5982,7 @@ _start:
 {
 lean_object* x_1; lean_object* x_2; lean_object* x_3; lean_object* x_4; lean_object* x_5; 
 x_1 = l___regBuiltin_Lean_Elab_Term_elabStrLit_declRange___closed__1;
-x_2 = lean_unsigned_to_nat(26u);
+x_2 = lean_unsigned_to_nat(23u);
 x_3 = l___regBuiltin_Lean_Elab_Term_elabStrLit_declRange___closed__2;
 x_4 = lean_unsigned_to_nat(36u);
 x_5 = lean_alloc_ctor(0, 4, 0);
@@ -5998,7 +5998,7 @@ _start:
 {
 lean_object* x_1; lean_object* x_2; lean_object* x_3; 
 x_1 = lean_unsigned_to_nat(165u);
-x_2 = lean_unsigned_to_nat(30u);
+x_2 = lean_unsigned_to_nat(27u);
 x_3 = lean_alloc_ctor(0, 2, 0);
 lean_ctor_set(x_3, 0, x_1);
 lean_ctor_set(x_3, 1, x_2);
@@ -6010,7 +6010,7 @@ _start:
 {
 lean_object* x_1; lean_object* x_2; lean_object* x_3; 
 x_1 = lean_unsigned_to_nat(165u);
-x_2 = lean_unsigned_to_nat(40u);
+x_2 = lean_unsigned_to_nat(37u);
 x_3 = lean_alloc_ctor(0, 2, 0);
 lean_ctor_set(x_3, 0, x_1);
 lean_ctor_set(x_3, 1, x_2);
@@ -6022,9 +6022,9 @@ _start:
 {
 lean_object* x_1; lean_object* x_2; lean_object* x_3; lean_object* x_4; lean_object* x_5; 
 x_1 = l___regBuiltin_Lean_Elab_Term_elabStrLit_declRange___closed__4;
-x_2 = lean_unsigned_to_nat(30u);
+x_2 = lean_unsigned_to_nat(27u);
 x_3 = l___regBuiltin_Lean_Elab_Term_elabStrLit_declRange___closed__5;
-x_4 = lean_unsigned_to_nat(40u);
+x_4 = lean_unsigned_to_nat(37u);
 x_5 = lean_alloc_ctor(0, 4, 0);
 lean_ctor_set(x_5, 0, x_1);
 lean_ctor_set(x_5, 1, x_2);
@@ -6533,7 +6533,7 @@ static lean_object* _init_l___regBuiltin_Lean_Elab_Term_elabNumLit___closed__1()
 _start:
 {
 lean_object* x_1; 
-x_1 = lean_mk_string("numLit");
+x_1 = lean_mk_string("num");
 return x_1;
 }
 }
@@ -6590,7 +6590,7 @@ _start:
 {
 lean_object* x_1; lean_object* x_2; lean_object* x_3; 
 x_1 = lean_unsigned_to_nat(177u);
-x_2 = lean_unsigned_to_nat(26u);
+x_2 = lean_unsigned_to_nat(23u);
 x_3 = lean_alloc_ctor(0, 2, 0);
 lean_ctor_set(x_3, 0, x_1);
 lean_ctor_set(x_3, 1, x_2);
@@ -6614,7 +6614,7 @@ _start:
 {
 lean_object* x_1; lean_object* x_2; lean_object* x_3; lean_object* x_4; lean_object* x_5; 
 x_1 = l___regBuiltin_Lean_Elab_Term_elabNumLit_declRange___closed__1;
-x_2 = lean_unsigned_to_nat(26u);
+x_2 = lean_unsigned_to_nat(23u);
 x_3 = l___regBuiltin_Lean_Elab_Term_elabNumLit_declRange___closed__2;
 x_4 = lean_unsigned_to_nat(10u);
 x_5 = lean_alloc_ctor(0, 4, 0);
@@ -6630,7 +6630,7 @@ _start:
 {
 lean_object* x_1; lean_object* x_2; lean_object* x_3; 
 x_1 = lean_unsigned_to_nat(177u);
-x_2 = lean_unsigned_to_nat(30u);
+x_2 = lean_unsigned_to_nat(27u);
 x_3 = lean_alloc_ctor(0, 2, 0);
 lean_ctor_set(x_3, 0, x_1);
 lean_ctor_set(x_3, 1, x_2);
@@ -6642,7 +6642,7 @@ _start:
 {
 lean_object* x_1; lean_object* x_2; lean_object* x_3; 
 x_1 = lean_unsigned_to_nat(177u);
-x_2 = lean_unsigned_to_nat(40u);
+x_2 = lean_unsigned_to_nat(37u);
 x_3 = lean_alloc_ctor(0, 2, 0);
 lean_ctor_set(x_3, 0, x_1);
 lean_ctor_set(x_3, 1, x_2);
@@ -6654,9 +6654,9 @@ _start:
 {
 lean_object* x_1; lean_object* x_2; lean_object* x_3; lean_object* x_4; lean_object* x_5; 
 x_1 = l___regBuiltin_Lean_Elab_Term_elabNumLit_declRange___closed__4;
-x_2 = lean_unsigned_to_nat(30u);
+x_2 = lean_unsigned_to_nat(27u);
 x_3 = l___regBuiltin_Lean_Elab_Term_elabNumLit_declRange___closed__5;
-x_4 = lean_unsigned_to_nat(40u);
+x_4 = lean_unsigned_to_nat(37u);
 x_5 = lean_alloc_ctor(0, 4, 0);
 lean_ctor_set(x_5, 0, x_1);
 lean_ctor_set(x_5, 1, x_2);
@@ -7269,7 +7269,7 @@ static lean_object* _init_l___regBuiltin_Lean_Elab_Term_elabScientificLit___clos
 _start:
 {
 lean_object* x_1; 
-x_1 = lean_mk_string("scientificLit");
+x_1 = lean_mk_string("scientific");
 return x_1;
 }
 }
@@ -7511,7 +7511,7 @@ static lean_object* _init_l___regBuiltin_Lean_Elab_Term_elabCharLit___closed__1(
 _start:
 {
 lean_object* x_1; 
-x_1 = lean_mk_string("charLit");
+x_1 = lean_mk_string("char");
 return x_1;
 }
 }
@@ -7568,7 +7568,7 @@ _start:
 {
 lean_object* x_1; lean_object* x_2; lean_object* x_3; 
 x_1 = lean_unsigned_to_nat(205u);
-x_2 = lean_unsigned_to_nat(27u);
+x_2 = lean_unsigned_to_nat(24u);
 x_3 = lean_alloc_ctor(0, 2, 0);
 lean_ctor_set(x_3, 0, x_1);
 lean_ctor_set(x_3, 1, x_2);
@@ -7592,7 +7592,7 @@ _start:
 {
 lean_object* x_1; lean_object* x_2; lean_object* x_3; lean_object* x_4; lean_object* x_5; 
 x_1 = l___regBuiltin_Lean_Elab_Term_elabCharLit_declRange___closed__1;
-x_2 = lean_unsigned_to_nat(27u);
+x_2 = lean_unsigned_to_nat(24u);
 x_3 = l___regBuiltin_Lean_Elab_Term_elabCharLit_declRange___closed__2;
 x_4 = lean_unsigned_to_nat(36u);
 x_5 = lean_alloc_ctor(0, 4, 0);
@@ -7608,7 +7608,7 @@ _start:
 {
 lean_object* x_1; lean_object* x_2; lean_object* x_3; 
 x_1 = lean_unsigned_to_nat(205u);
-x_2 = lean_unsigned_to_nat(31u);
+x_2 = lean_unsigned_to_nat(28u);
 x_3 = lean_alloc_ctor(0, 2, 0);
 lean_ctor_set(x_3, 0, x_1);
 lean_ctor_set(x_3, 1, x_2);
@@ -7620,7 +7620,7 @@ _start:
 {
 lean_object* x_1; lean_object* x_2; lean_object* x_3; 
 x_1 = lean_unsigned_to_nat(205u);
-x_2 = lean_unsigned_to_nat(42u);
+x_2 = lean_unsigned_to_nat(39u);
 x_3 = lean_alloc_ctor(0, 2, 0);
 lean_ctor_set(x_3, 0, x_1);
 lean_ctor_set(x_3, 1, x_2);
@@ -7632,9 +7632,9 @@ _start:
 {
 lean_object* x_1; lean_object* x_2; lean_object* x_3; lean_object* x_4; lean_object* x_5; 
 x_1 = l___regBuiltin_Lean_Elab_Term_elabCharLit_declRange___closed__4;
-x_2 = lean_unsigned_to_nat(31u);
+x_2 = lean_unsigned_to_nat(28u);
 x_3 = l___regBuiltin_Lean_Elab_Term_elabCharLit_declRange___closed__5;
-x_4 = lean_unsigned_to_nat(42u);
+x_4 = lean_unsigned_to_nat(39u);
 x_5 = lean_alloc_ctor(0, 4, 0);
 lean_ctor_set(x_5, 0, x_1);
 lean_ctor_set(x_5, 1, x_2);
