git/tylerhanks/AwodeyCT/AwodeyCT.lean
@@ -159,7 +159,7 @@ class Preorder (Ob : Type u) where
   leq_trans : ∀ a b c : Ob, (leq a b) → (leq b c) → (leq a c)
   leq_decidable : ∀ a b : Ob, Decidable (leq a b)
 
-/-instance NatPreorder : Preorder Nat where
+instance NatPreorder : Preorder Nat where
   leq := Nat.le
   leq_ref := by simp 
   leq_trans := by 
@@ -167,7 +167,7 @@ class Preorder (Ob : Type u) where
     apply Nat.le_trans
   leq_decidable a b := by
     simp
-    apply Nat.decLe-/
+    apply Nat.decLe
 
 instance NatMod4Preorder : Preorder Nat where
   leq a b := a / 4 ≤ b / 4
@@ -186,21 +186,22 @@ instance NatMod4Preorder : Preorder Nat where
 
 --#check NatPreorder.leq
 
---#eval NatPreorder.leq 5 7 -- false
---#eval Nat.ble_eq_true_of_le (NatMod4Preorder.leq 3 0) -- true
+--#eval NatPreorder.leq 3 0 -- false
+--#eval NatMod4Preorder.leq 3 0 -- true
 
 --structure monotone_map (C : Type u₁) (D : Type u₂) [Preorder C] [Preorder D] where
 
-structure bottom (C : Type u) [Preorder C] where
+structure bottom (C : Type u) (P : Preorder C) where
   bot : C
-  is_bottom : ∀ x : C, Preorder.leq bot x
+  is_bottom : ∀ x : C, P.leq bot x
 
--- Something is wrong because I can "prove" that 0 is the bottom of this cyclic preorder with no bottoms :(
-def nat_bottom : bottom Nat := {
+def nat_bottom : bottom Nat NatMod4Preorder := {
   bot := 0
   is_bottom := by
     intro x
+    --show 0 / 4 ≤ x / 4
     apply Nat.zero_le
+    
 }
 
 #check nat_bottom
@@ -214,7 +215,27 @@ structure has_all_joins (C : Type u) (P : Preorder C) where
   pf : ∀ (a b : C), ∃ (j : C),
     (P.leq a j) ∧ (P.leq b j) ∧ (∀ x : C, (P.leq a x) → (P.leq b x) → (P.leq j x))
 
---theorem bottom_implies_all_joins : ∀ (C : Type u) [Preorder C]
+structure meet (C : Type u) (a b : C) (P : Preorder C) where
+  m : C
+  lower_bound : (P.leq m a) ∧ (P.leq m b)
+  greatest: ∀ x : C, (P.leq x a) → (P.leq x b) → (P.leq x m)
+
+structure has_all_meets (C : Type u) (P : Preorder C) where
+  pf : ∀ (a b : C), ∃ (m : C),
+    (P.leq m a) ∧ (P.leq m b) ∧ (∀ x : C, (P.leq x a) → (P.leq x b) → (P.leq x m))
+
+open Classical
+theorem bottom_implies_all_meets : ∀ (C : Type u) [P : Preorder C],
+  (bottom C P) → (has_all_meets C P) := by
+    intros C P bot
+    induction bot
+
+    constructor
+    intros a b
+    
+    
+    
+    
 
 
 end PreorderCats
